Rename tio to iodiv

Itree.fst
@@ -698,14 +698,14 @@ let rec ipos_trace_append (p q : iopos) :
   | Call_choice o x y :: p -> ipos_trace_append p q
 
 unfold
-let tio_post a = trace -> option a -> Type0
+let iodiv_post a = trace -> option a -> Type0
 
-let twp a = tio_post a -> Type0
+let twp a = iodiv_post a -> Type0
 
 let twp_return #a (x : a) : twp a =
   fun post -> post [] (Some x)
 
-let shift_post #a (tr : trace) (post : tio_post a) : tio_post a =
+let shift_post #a (tr : trace) (post : iodiv_post a) : iodiv_post a =
   fun tr' x -> post (tr @ tr') x
 
 let twp_bind #a #b (w : twp a) (f : a -> twp b) : twp b =
@@ -724,50 +724,50 @@ let io_twp #a (t : iotree a) =
     (forall p. isRet (t p) ==> post (ipos_trace p) (Some (ret_val (t p)))) /\
     (forall p. isEvent (t p) ==> post (ipos_trace p) None)
 
-let tio a (w : twp a) =
+let iodiv a (w : twp a) =
   t: iotree a { w `stronger_twp` io_twp t }
 
-let tio_return a (x : a) : tio a (twp_return x) =
+let iodiv_return a (x : a) : iodiv a (twp_return x) =
   ret x
 
-let tio_bind a b w wf (m : tio a w) (f : (x:a) -> tio b (wf x)) : tio b (twp_bind w wf) =
-  assert (forall (post : tio_post a). w post ==> io_twp m post) ;
-  assert (forall (post : tio_post b) x. wf x post ==> io_twp (f x) post) ;
+let iodiv_bind a b w wf (m : iodiv a w) (f : (x:a) -> iodiv b (wf x)) : iodiv b (twp_bind w wf) =
+  assert (forall (post : iodiv_post a). w post ==> io_twp m post) ;
+  assert (forall (post : iodiv_post b) x. wf x post ==> io_twp (f x) post) ;
 
   // ret
   forall_intro (find_ret_Some_pos m []) ;
   forall_intro_2 ipos_trace_append ;
   forall_intro (find_ret_prefix_val m []) ;
-  assert (forall (post : tio_post b) p. twp_bind w wf post ==> isRet (bind m f p) ==> post (ipos_trace p) (Some (ret_val (bind m f p)))) ;
+  assert (forall (post : iodiv_post b) p. twp_bind w wf post ==> isRet (bind m f p) ==> post (ipos_trace p) (Some (ret_val (bind m f p)))) ;
 
   // event.ret
-  assert (forall (post : tio_post b) p. twp_bind w wf post ==> isEvent (bind m f p) ==> Some? (find_ret m [] p) ==> post (ipos_trace p) None) ;
+  assert (forall (post : iodiv_post b) p. twp_bind w wf post ==> isEvent (bind m f p) ==> Some? (find_ret m [] p) ==> post (ipos_trace p) None) ;
 
   // event.noret
-  assert (forall (post : tio_post b) p.
+  assert (forall (post : iodiv_post b) p.
     twp_bind w wf post ==>
     isEvent (bind m f p) ==>
     None? (find_ret m [] p) ==>
     isEvent (m p)
   ) ;
-  assert (forall (post : tio_post b) p. twp_bind w wf post ==> isEvent (bind m f p) ==> None? (find_ret m [] p) ==> post (ipos_trace p) None) ;
+  assert (forall (post : iodiv_post b) p. twp_bind w wf post ==> isEvent (bind m f p) ==> None? (find_ret m [] p) ==> post (ipos_trace p) None) ;
 
   // event
-  assert (forall (post : tio_post b) p. twp_bind w wf post ==> isEvent (bind m f p) ==> post (ipos_trace p) None) ;
+  assert (forall (post : iodiv_post b) p. twp_bind w wf post ==> isEvent (bind m f p) ==> post (ipos_trace p) None) ;
 
-  assert (forall (post : tio_post b). twp_bind w wf post ==> io_twp (bind m f) post) ;
+  assert (forall (post : iodiv_post b). twp_bind w wf post ==> io_twp (bind m f) post) ;
   bind m f
 
 let twp_tau #a (w : twp a) : twp a =
   fun post -> post [] None /\ w post
 
-let tio_tau #a #w (m : tio a w) : tio a (twp_tau w) =
+let iodiv_tau #a #w (m : iodiv a w) : iodiv a (twp_tau w) =
   tau m
 
 let twp_call #a (o : cmds) (x : io_args o) (w : io_res o -> twp a) : twp a =
   fun post -> post [] None /\ (forall y. w y (shift_post [ Call_choice o x y ] post))
 
-let tio_call #a (o : cmds) (x : io_args o) #w (k : (r : io_res o) -> tio a (w r)) : tio a (twp_call o x w) =
+let iodiv_call #a (o : cmds) (x : io_args o) #w (k : (r : io_res o) -> iodiv a (w r)) : iodiv a (twp_call o x w) =
   call o x k
 
 let rec twp_repeat_trunc (w : twp unit) (n : nat) : twp unit =
@@ -833,10 +833,10 @@ let rec repeat_any_ret (body : iotree unit) (pl : list iopos) p :
       repeat body p ;
     }
 
-let rec repeat_any_ret_event_post #w (body : tio unit w) (pl : list iopos) p :
+let rec repeat_any_ret_event_post #w (body : iodiv unit w) (pl : list iopos) p :
   Lemma
     (requires forall pp. mem pp pl ==> isRet (body pp))
-    (ensures forall (post : tio_post unit).
+    (ensures forall (post : iodiv_post unit).
       twp_repeat_trunc w (1 + length pl) post ==>
       isEvent (body p) ==>
       post (ipos_trace (flatten_sep [Tau_choice] pl @ p)) None
@@ -858,10 +858,10 @@ let rec repeat_any_ret_event_post #w (body : tio unit w) (pl : list iopos) p :
       ipos_trace pp @ ipos_trace (flatten_sep [Tau_choice] pl @ p) ;
     }
 
-let rec repeat_any_ret_ret_post #w (body : tio unit w) (pl : list iopos) p :
+let rec repeat_any_ret_ret_post #w (body : iodiv unit w) (pl : list iopos) p :
   Lemma
     (requires forall pp. mem pp pl ==> isRet (body pp))
-    (ensures forall (post : tio_post unit).
+    (ensures forall (post : iodiv_post unit).
       twp_repeat_trunc w (1 + length pl) post ==>
       isRet (body p) ==>
       post (ipos_trace (flatten_sep [Tau_choice] pl @ p)) None
@@ -869,19 +869,19 @@ let rec repeat_any_ret_ret_post #w (body : tio unit w) (pl : list iopos) p :
     (decreases pl)
 = match pl with
   | [] ->
-    assert (forall (post : tio_post unit).
+    assert (forall (post : iodiv_post unit).
       twp_repeat_trunc w 1 post ==>
       isRet (body p) ==>
       twp_tau (twp_repeat_trunc w 0) (shift_post (ipos_trace p) post)
     )
   | pp :: pl ->
     repeat_any_ret_ret_post body pl p ;
-    assert (forall (post : tio_post unit).
+    assert (forall (post : iodiv_post unit).
       twp_repeat_trunc w (1 + length pl) post ==>
       isRet (body p) ==>
       post (ipos_trace (flatten_sep [Tau_choice] pl @ p)) None
     ) ;
-    assert (forall (post : tio_post unit).
+    assert (forall (post : iodiv_post unit).
       twp_repeat_trunc w (1 + length pl) (shift_post (ipos_trace pp) post) ==>
       isRet (body p) ==>
       shift_post (ipos_trace pp) post (ipos_trace (flatten_sep [Tau_choice] pl @ p)) None
@@ -897,21 +897,21 @@ let rec repeat_any_ret_ret_post #w (body : tio unit w) (pl : list iopos) p :
       == {}
       ipos_trace pp @ ipos_trace (flatten_sep [Tau_choice] pl @ p) ;
     } ;
-    assert (forall (post : tio_post unit).
+    assert (forall (post : iodiv_post unit).
       twp_repeat_trunc w (1 + length pl) (shift_post (ipos_trace pp) post) ==>
       isRet (body p) ==>
       post (ipos_trace (flatten_sep [Tau_choice] (pp :: pl) @ p)) None
     ) ;
-    assert (forall (post : tio_post unit).
+    assert (forall (post : iodiv_post unit).
       twp_repeat_trunc w (2 + length pl) post ==>
       isRet (body p) ==>
       post (ipos_trace (flatten_sep [Tau_choice] (pp :: pl) @ p)) None
     )
 
-let rec tio_repeat_proof_gen #w (body : tio unit w) (pl : list iopos) p :
+let rec iodiv_repeat_proof_gen #w (body : iodiv unit w) (pl : list iopos) p :
   Lemma
     (requires forall pp. mem pp pl ==> isRet (body pp))
-    (ensures forall (post : tio_post unit).
+    (ensures forall (post : iodiv_post unit).
       twp_repeat w post ==>
       isEvent (repeat body (flatten_sep [Tau_choice] pl @ p)) ==>
       post (ipos_trace (flatten_sep [Tau_choice] pl @ p)) None
@@ -929,8 +929,8 @@ let rec tio_repeat_proof_gen #w (body : tio unit w) (pl : list iopos) p :
       assert (repeat body p == Some Tau) ;
       repeat_any_ret_ret_post body pl p ;
       assert (isRet (body p)) ;
-      assert (forall (post : tio_post unit). twp_repeat w post ==> twp_repeat_trunc w (1 + length pl) post) ;
-      assert (forall (post : tio_post unit).
+      assert (forall (post : iodiv_post unit). twp_repeat w post ==> twp_repeat_trunc w (1 + length pl) post) ;
+      assert (forall (post : iodiv_post unit).
         twp_repeat w post ==>
         isEvent (repeat body p) ==>
         post (ipos_trace (flatten_sep [Tau_choice] pl @ p)) None
@@ -946,41 +946,41 @@ let rec tio_repeat_proof_gen #w (body : tio unit w) (pl : list iopos) p :
       flatten_sep_nil #iochoice [Tau_choice] ;
       assert (flatten_sep [Tau_choice] pl @ p == flatten_sep [Tau_choice] (pl @ [find_ret_prefix body [] p]) @ r) ;
       find_ret_smaller body [] p ;
-      tio_repeat_proof_gen body (pl @ [find_ret_prefix body [] p]) r
+      iodiv_repeat_proof_gen body (pl @ [find_ret_prefix body [] p]) r
     | c :: r -> repeat_any_ret body pl p ; repeat_unfold_1 body
     end
   | None ->
     repeat_any_ret body pl p ;
     repeat_any_ret_event_post body pl p ;
-    assert (forall (post : tio_post unit). twp_repeat w post ==> twp_repeat_trunc w (1 + length pl) post) ;
+    assert (forall (post : iodiv_post unit). twp_repeat w post ==> twp_repeat_trunc w (1 + length pl) post) ;
     repeat_unfold_1 body ;
     assert (
       isEvent (repeat body p) ==> isEvent (body p)
     ) ;
-    assert (forall (post : tio_post unit).
+    assert (forall (post : iodiv_post unit).
       twp_repeat w post ==>
       isEvent (repeat body p) ==>
       post (ipos_trace (flatten_sep [Tau_choice] pl @ p)) None
     )
 
-let tio_repeat_proof #w (body : tio unit w) p :
-  Lemma (forall (post : tio_post unit).
+let iodiv_repeat_proof #w (body : iodiv unit w) p :
+  Lemma (forall (post : iodiv_post unit).
     twp_repeat w post ==>
     isEvent (repeat body p) ==>
     post (ipos_trace p) None
   )
-= tio_repeat_proof_gen body [] p
+= iodiv_repeat_proof_gen body [] p
 
-let tio_repeat #w (body : tio unit w) : tio unit (twp_repeat w) =
+let iodiv_repeat #w (body : iodiv unit w) : iodiv unit (twp_repeat w) =
   forall_intro (repeat_not_ret body) ;
-  forall_intro (tio_repeat_proof body) ;
+  forall_intro (iodiv_repeat_proof body) ;
   repeat body
 
 // We can also "inline" the induction by asking the SMT to prove (p n ==> p (n+1)) which might work sometimes
 
 (**
 
-  Alternatively, we propose a definition of tio_repeat using an invariant.
+  Alternatively, we propose a definition of iodiv_repeat using an invariant.
   The invariant is relative to the predicate transformer of the body.
   It must hold for the empty list / root position because postconditions
   must be downward closed.
@@ -994,7 +994,7 @@ let trace_invariant (w : twp unit) (inv : trace -> Type0) =
 let twp_repeat_with_inv (w : twp unit) (inv : trace -> Type0) : twp unit =
   fun post -> forall tr. inv tr ==> post tr None
 
-let invpost (inv : trace -> Type0) : tio_post unit =
+let invpost (inv : trace -> Type0) : iodiv_post unit =
   fun tr v -> inv tr /\ None? v
 
 let rec twp_repeat_inv_trunc (w : twp unit) (inv : trace -> Type0) n :
@@ -1018,7 +1018,7 @@ let rec twp_repeat_inv_trunc (w : twp unit) (inv : trace -> Type0) n :
       //   | None -> invpost inv tr None // == inv tr
       // )
     ) ;
-    assume (forall (post : tio_post unit).
+    assume (forall (post : iodiv_post unit).
       twp_bind w (fun (_:unit) -> twp_tau (twp_repeat_trunc w (n - 1))) post ==>
       twp_repeat_trunc w n post
     ) ; // why??
@@ -1032,16 +1032,16 @@ let rec twp_repeat_inv_trunc (w : twp unit) (inv : trace -> Type0) n :
 // Some specifications
 
 // Does not make sense at the moment
-// let terminates #a : tio_post a =
+// let terminates #a : iodiv_post a =
 //   fun tr v -> Some? v
 
-let diverges #a : tio_post a =
+let diverges #a : iodiv_post a =
   fun tr v -> None? v
 
 // let ret_terminates a (x : a) : Lemma (twp_return x terminates) = ()
 
 // Should be p1 ==> p2 rather than ==
-let rec twp_repeat_trunc_ext w n (p1 p2 : tio_post unit) :
+let rec twp_repeat_trunc_ext w n (p1 p2 : iodiv_post unit) :
   Lemma ((forall tr x. p1 tr x == p2 tr x) ==> twp_repeat_trunc w n p1 == twp_repeat_trunc w n p2)
 = if n = 0
   then ()
@@ -1074,9 +1074,9 @@ let repeat_ret_loops_with_inv () :
 reifiable total layered_effect {
   IODiv : a:Type -> twp a -> Effect
   with
-    repr   = tio ;
-    return = tio_return ;
-    bind   = tio_bind
-    // tau    = tio_tau ; // Universe problems
-    // call   = tio_call
+    repr   = iodiv ;
+    return = iodiv_return ;
+    bind   = iodiv_bind
+    // tau    = iodiv_tau ; // Universe problems
+    // call   = iodiv_call
 }
